src/example.lean
@@ -1,6 +1,8 @@
 import tactic.gptf
 import data.list.sigma
 
+section gptf
+
 example {α} (a : α) : a = a :=
 begin
   refl
@@ -58,3 +60,67 @@ example {α : Type u} {β : α → Type v} [_inst_1 : decidable_eq α] {a : α} 
 begin
   induction l₁ with x xs generalizing l₂; cases l₂ with y ys; simp
 end
+
+end gptf
+
+section gptf_exact
+
+example {α} (a : α) : a = a :=
+begin
+  exact (rfl)
+end
+
+example : ∃ n : ℕ, 8 = 2*n :=
+begin
+  exact (of_as_true trivial)
+end
+
+example {P Q R : Prop} : P → (P → R) → R :=
+begin
+  exact (λ (h1 : P) (h2 : P → R), h2 h1)
+end
+
+example {p q r : Prop} (h₁ : p) (h₂ : q) : (p ∧ q) ∨ r :=
+begin
+  exact (or.inl ⟨h₁, h₂⟩)
+end
+
+example {P Q : Prop} : (¬ P) ∧ (¬ Q) → ¬ (P ∨ Q) :=
+begin
+  exact (not_or_distrib.mpr)
+end
+
+example {P Q R : Prop} : (P ∧ Q) → ((P → R) → ¬ (Q → ¬ R)) :=
+begin
+  refine (λ (h₁ : P ∧ Q) (h₂ : P → R), _),
+  intro h₃, apply h₃ h₁.2, exact (h₂ h₁.left)
+end
+
+example (n : ℕ) (m : ℕ) : nat.succ n < nat.succ n + 1  :=
+begin
+  exact (nat.lt_succ_iff.mpr n.lt_succ_self)
+end
+
+example : ∀ (F1 F2 F3 : Prop), ((¬F1 ∧ F3) ∨ (F2 ∧ ¬F3)) → (F2 → F1) → (F2 → F3) →  ¬F2 :=
+begin
+  tauto
+end
+
+example : ∀ (f : nat → Prop), f 2 → ∃ x, f x :=
+begin
+  exact (λ (f : ℕ → Prop) (h : f 2), Exists.intro 2 h)
+end
+
+example {G} [group G] (x y z : G) : (x * z) * (z⁻¹ * y) = x * y :=
+begin
+  simp [mul_assoc]
+end
+universes u v
+
+example {α : Type u} {β : α → Type v} [_inst_1 : decidable_eq α] {a : α} {l₁ l₂ : list (sigma β)} :
+  (list.kerase a l₁).kunion (list.kerase a l₂) = list.kerase a (l₁.kunion l₂) :=
+begin
+  exact (list.kunion_kerase)
+end
+
+end gptf_exact
